Main.lean
@@ -1,9 +1,12 @@
+import Mica.TinyML.Typed
 import Mica.TinyML.Printer
 import Mica.Frontend.Parser
 import Mica.Frontend.Printer
 import Mica.Frontend.Elaborate
 import Mica.Verifier.Programs
 import Mica.Engine.Driver
+
+open Typed
 
 private def bold (s : String) : String := s!"\x1b[1m{s}\x1b[0m"
 
@@ -49,13 +52,14 @@ def main (args : List String) : IO Unit := do
         IO.Process.exit 1
     if opts.printOcaml then
       IO.println (Frontend.Program.print frontendProg)
-    let prog ← match Frontend.Program.elaborate frontendProg with
+    let untypedProg ← match Frontend.Program.elaborate frontendProg with
       | .ok prog => pure prog
       | .error e => do
         IO.eprintln s!"elaboration error: {e}"
         IO.Process.exit 1
+    let prog := Typed.Program.elaborate untypedProg
     if opts.printTinyML then
-      IO.println (TinyML.Program.print prog)
+      IO.println (Program.print prog)
     if opts.noCheck then
       return
     let strategy := Program.verify prog
