Mica/TinyML.lean
@@ -1,3 +1,5 @@
-import Mica.TinyML.Expr
+import Mica.TinyML.Common
+import Mica.TinyML.Untyped
+import Mica.TinyML.Typed
 import Mica.TinyML.Printer
 import Mica.TinyML.WeakestPre
